WIP: computable validity

src/Bedrock/Proofs/ValidComputable.v
@@ -63,7 +63,7 @@ Section Expr.
     | _ => false
     end.
   
-  Definition valid_expr_App2_bool {t} (require_casts : bool)
+  Definition valid_expr_binop_bool {t} (require_casts : bool)
            (e : @API.expr (fun _ => unit) t) : bool :=
     match e with
     | expr.App
@@ -151,36 +151,65 @@ Section Expr.
     | _ => false
     end.
 
-  Fixpoint valid_expr_bool {t} (require_casts : bool)
-             (e : @API.expr (fun _ => unit) t) {struct e} : bool :=
-    match e with
-    | expr.App type_nat _ f x =>
-      (* only thing accepting nat is nth_default *)
-      if require_casts
-      then false
-      else valid_expr_nth_default_bool (expr.App f x)
-    | expr.App type_Z type_Z
-               (expr.App type_Z _ f x) y =>
-      if valid_expr_App2_bool require_casts f
-      then valid_expr_bool true x && valid_expr_bool true y
-      else if valid_expr_shift_bool require_casts f
-           then valid_expr_bool true x && valid_shifter y
-           else false
-    | expr.App type_Z type_Z f x =>
-      valid_expr_App1_bool require_casts f && valid_expr_bool true x
-    | expr.App type_ZZ type_Z f x =>
-      valid_expr_App1_bool require_casts f && valid_expr_bool true x
-    | expr.App type_ZZ type_ZZ f x =>
-      valid_expr_App1_bool require_casts f && valid_expr_bool true x
-    | expr.Ident _ (ident.Literal base.type.Z z) =>
-      negb require_casts || is_bounded_by_bool z max_range
-    | expr.Ident _ (ident.Literal base.type.nat n) =>
-      negb require_casts
-    | expr.Var type_Z v => negb require_casts
-    | expr.Var type_listZ v => true
-    | _ => false
-    end.
- 
+  (* add an extra flag to translate binops because otherwise the inductive
+     hypothesis won't be strong enough to give information about *both*
+     arguments to a binop *)
+  Fixpoint valid_expr_bool' {t}
+           (binop_only shift_only require_casts : bool)
+           (e : @API.expr (fun _ => unit) t) {struct e} : bool :=
+    if binop_only
+    then match e with
+         | expr.App type_Z (type.arrow type_Z type_Z) f x =>
+           (valid_expr_binop_bool require_casts f)
+             && valid_expr_bool' false false true x
+         | _ => false
+         end
+    else
+      if shift_only
+      then match e with
+           | expr.App type_Z (type.arrow type_Z type_Z) f x =>
+             (valid_expr_shift_bool require_casts f)
+               && valid_expr_bool' false false true x
+           | _ => false
+           end
+      else 
+        match e with
+        | expr.App type_nat _ f x =>
+          (* only thing accepting nat is nth_default *)
+          if require_casts
+          then false
+          else valid_expr_nth_default_bool (expr.App f x)
+        | expr.App type_Z type_Z f x =>
+          if valid_expr_bool' true false require_casts f
+          then (* f is a binop applied to one valid argument;
+                check that x (second argument) is also valid *)
+            valid_expr_bool' false false true x
+          else if valid_expr_bool' false true require_casts f
+               then (* f is a shift applied to one valid
+                       argument; check that x (shifting index) is a
+                       valid shifter *)
+                 valid_shifter x
+               else (* must be a cast *)
+                 (valid_expr_App1_bool require_casts f)
+                   && valid_expr_bool' false false false x
+        | expr.App type_ZZ type_Z f x =>
+          (* fst or snd *)
+          (valid_expr_App1_bool require_casts f)
+            && valid_expr_bool' false false true x
+        | expr.App type_ZZ type_ZZ f x =>
+          (valid_expr_App1_bool require_casts f)
+            && valid_expr_bool' false false false x
+        | expr.Ident _ (ident.Literal base.type.Z z) =>
+          negb require_casts || is_bounded_by_bool z max_range
+        | expr.Ident _ (ident.Literal base.type.nat n) =>
+          negb require_casts
+        | expr.Var type_Z v => negb require_casts
+        | expr.Var type_listZ v => true
+        | _ => false
+        end.
+
+  Definition valid_expr_bool {t} := @valid_expr_bool' t false false.
+
   Lemma valid_expr_App1_bool_type {t} rc (e : API.expr t) :
     valid_expr_App1_bool rc e = true ->
     (exists d,
@@ -227,12 +256,12 @@ Section Expr.
     break_match; congruence.
   Qed.
 
-  Lemma valid_expr_App2_bool_type {t} rc (f : API.expr t) :
-    valid_expr_App2_bool rc f = true ->
+  Lemma valid_expr_binop_bool_type {t} rc (f : API.expr t) :
+    valid_expr_binop_bool rc f = true ->
     t = type.arrow type_Z
                    (type.arrow type_Z type_Z).
   Proof.
-    cbv [valid_expr_App2_bool translate_binop].
+    cbv [valid_expr_binop_bool translate_binop].
     destruct f;
       match goal with
       | idc : ident.ident _ |- _ =>
@@ -620,9 +649,9 @@ Section Expr.
     congruence.
   Qed.
 
-  Lemma valid_expr_App2_bool_impl1 {t}
+  Lemma valid_expr_binop_bool_impl1 {t}
         rc (f : API.expr t) :
-    valid_expr_App2_bool rc f = true ->
+    valid_expr_binop_bool rc f = true ->
     (match t as t0 return expr.expr t0 -> Prop with
      | type.arrow type_Z (type.arrow type_Z type_Z) =>
        fun f =>
@@ -633,7 +662,7 @@ Section Expr.
      | _ => fun _ => False
      end) f.
   Proof.
-    cbv [valid_expr_App2_bool].
+    cbv [valid_expr_binop_bool].
     break_match; try congruence; [ | ];
       intros;
       repeat match goal with
@@ -729,66 +758,33 @@ Section Expr.
       constructor; eauto; lia. }
   Qed.
 
-  Lemma valid_expr_App_bool_impl1 {t} rc
-        (f : API.expr t) (y : API.expr type_Z) :
-    match f with
-    | expr.App type_Z _ f x =>
-      if valid_expr_App2_bool rc f
-      then valid_expr_bool true x && valid_expr_bool true y
-      else if valid_expr_shift_bool rc f
-           then valid_expr_bool true x && valid_shifter y
-           else false
-    | _ => false
-    end = true ->
-    (match t as t0 return expr.expr t0 -> Prop with
-     | type.arrow type_Z type_Z =>
-       fun f =>
-           valid_expr true y ->
-           valid_expr rc (expr.App f y)
-     | type.arrow type_ZZ _ =>
-       fun f =>
-         forall y,
-           valid_expr true y ->
-           valid_expr rc (expr.App f y)
-     | _ => fun _ => False
-     end) f.
-  Proof.
-    intro. remember t.
-    break_match;
-      try match goal with
-          | |- forall (_:false = true), _ => congruence
-          | H : valid_expr_App2_bool _ _ = true |- _ =>
-            apply valid_expr_App2_bool_type in H;
-              congruence
-          | H : valid_expr_shift_bool _ _ = true |- _ =>
-            apply valid_expr_shift_bool_type in H;
-              congruence
-          end; [ | ].
-    { intros;
-        repeat match goal with
-               | H : _ && _ = true |- _ =>
-                 apply andb_true_iff in H; destruct H
-               | H : valid_expr_App2_bool _ _ = true |- _ =>
-                 apply valid_expr_App2_bool_impl1 in H
-               end.
-      eauto. }
-    { intros; 
-        repeat match goal with
-               | H : _ && _ = true |- _ =>
-                 apply andb_true_iff in H; destruct H
-               | H : valid_expr_shift_bool _ _ = true |- _ =>
-                 apply valid_expr_shift_bool_impl1 in H
-               end.
-      eauto. }
-  Qed.
-
-  Lemma valid_expr_bool_impl1 {t} (e : API.expr t) :
-    (exists b, t = type.base b) ->
-    forall rc,
-      valid_expr_bool rc e = true -> valid_expr rc e.
+  Lemma valid_expr_bool'_impl1 {t} (e : API.expr t) :
+    forall binop_only shift_only rc,
+      valid_expr_bool' binop_only shift_only rc e = true ->
+      if binop_only
+      then (match t as t0 return expr.expr t0 -> Prop with
+            | type.arrow type_Z type_Z =>
+              fun f =>
+                forall x,
+                  valid_expr true x -> 
+                  valid_expr rc (expr.App f x)
+            | _ => fun _ => False
+            end) e
+      else if shift_only
+           then (match t as t0 return expr.expr t0 -> Prop with
+                 | type.arrow type_Z type_Z =>
+                   fun f =>
+                     forall x,
+                       valid_shifter x = true -> 
+                       valid_expr rc (expr.App f x)
+                 | _ => fun _ => False
+                 end) e
+           else
+             (exists b, t = type.base b) -> valid_expr rc e.
   Proof.
     induction e; intros;
-      cbn [valid_expr_bool] in *.
+      cbn [valid_expr_bool'] in *;
+      [ | | | | ].
     { break_match_hyps; try congruence.
       { constructor.
         repeat match goal with
@@ -807,6 +803,7 @@ Section Expr.
       { constructor. } }
     { break_match_hyps; congruence. }
     { remember s.
+      remember d.
       break_match_hyps; try congruence;
           repeat match goal with
                  | H : _ && _ = true |- _ =>
@@ -814,807 +811,53 @@ Section Expr.
                  | H: valid_expr_App1_bool _ _ = true |- _ =>
                    apply valid_expr_App1_bool_type in H;
                      destruct H; destruct H; congruence
-                 end; [ | | | ].
-      { apply (@valid_expr_App_bool_impl1 (type.arrow type_Z type_Z)).
-        { 
-        break_match; try congruence;
-          repeat match goal with
-                 | H : _ && _ = true |- _ =>
-                   apply andb_true_iff in H; destruct H
-                 | _ => assumption
-                 end. }
-      { eauto using valid_expr_nth_default_bool_impl1. }
-      { pose proof H0.
-        apply valid_expr_App1_bool_type in H0.
-        destruct H0. destruct H0; try congruence.
-        inversion H0; subst.
-        (* need valid_expr_App1_bool_impl1 like nth_default model *)
-        (* probably get rid of current valid_expr_App_bool_impl1? *)
-
-  Fixpoint valid_expr_bool {t} (require_casts : bool)
-             (e : @API.expr (fun _ => unit) t) : bool :=
-    match e with
-    | expr.App
-        (expr.Ident _ (ident.Literal base.type.zrange r))) x =>
-      range_good r && valid_expr_bool false x
-    | expr.App
-        _ _
-        (expr.App
-           _ _ (expr.Ident _ ident.Z_cast2)
-           (expr.App
-              _ _
-              (expr.App
-                 _ _
-                 (expr.Ident _ (ident.pair _ _))
-                 (expr.Ident _ (ident.Literal base.type.zrange r1)))
-              (expr.Ident _ (ident.Literal base.type.zrange r2)))) x =>
-      range_good r1 && range_good r2 && valid_expr_bool false x
-    | expr.App _ _ (expr.Ident _ (ident.fst _ _)) x =>
-      negb require_casts && valid_expr_bool true x
-    | expr.App _ _ (expr.Ident _ (ident.snd _ _)) x =>
-      negb require_casts && valid_expr_bool true x
-    | expr.Ident _ (ident.Literal base.type.Z z) =>
-      negb require_casts || is_bounded_by_bool z max_range
-    | expr.Ident _ (ident.Literal base.type.nat n) =>
-      negb require_casts
-    | expr.Var type_Z v => negb require_casts
-    | expr.Var type_listZ v => true
-    | expr.App
-        _ _ (expr.App
-               _ _ (expr.App
-                      _ _ (expr.Ident _ (ident.List_nth_default _)) d)
-               (expr.Var type_listZ l))
-        (expr.Ident _ (ident.Literal base.type.nat i)) =>
-      negb require_casts && valid_expr_bool true d
-    | expr.App
-        _ _ (expr.App
-               _ _ (expr.Ident _ ident.Z_shiftr) x)
-        (expr.Ident _ (ident.Literal base.type.Z n)) =>
-      negb require_casts && is_bounded_by_bool n width_range
-           && valid_expr_bool true x
-    | expr.App
-        _ _ (expr.App
-               _ _ (expr.App
-                      _ _ (expr.Ident _ ident.Z_mul_high)
-                      (expr.Ident _ (ident.Literal base.type.Z s)))
-               x) y =>
-      negb require_casts && Z.eqb s (2 ^ Semantics.width)
-           && valid_expr_bool true x && valid_expr_bool true y
-    | expr.App
-        _ _ (expr.App
-               _ _ (expr.App
-                      _ _ (expr.Ident _ ident.Z_truncating_shiftl)
-                      (expr.Ident _ (ident.Literal base.type.Z s)))
-               x)
-        (expr.Ident _ (ident.Literal base.type.Z n)) =>
-      negb require_casts && is_bounded_by_bool n width_range
-           && Z.eqb s Semantics.width && valid_expr_bool true x
-    | expr.App
-        _ _ (expr.App _ _ (expr.Ident _ i) x) y =>
-      match translate_binop i with
-      | None => false
-      | Some _ =>
-        negb require_casts && valid_expr_bool true x
-             && valid_expr_bool true y
-      end
-    | _ => false
-    end.
-  (* TODO: remove nat case *)
-
-
-  Lemma valid_expr_bool_impl1 {t} (e : API.expr t) :
-    forall rc,
-      valid_expr_bool rc e = true -> valid_expr rc e.
-  Proof.
-    induction e; intros;
-      cbn [valid_expr_bool] in *.
-    { break_match_hyps; try congruence.
-      { constructor.
-        repeat match goal with
-               | _ => progress cbn [orb]
-               | H : _ || _ = true |- _ =>
-                 apply orb_true_iff in H; destruct H
-               | H : _ = true |- _ => rewrite H
-               | _ => rewrite Bool.orb_true_r
-               | _ => reflexivity
-               end. }
-      { destruct rc; cbn [negb] in *; try congruence.
-        constructor. } }
-    { break_match_hyps; try congruence.
-      { destruct rc; cbn [negb] in *; try congruence.
-        constructor. }
-      { constructor. } }
-    { break_match_hyps; try congruence. }
-    { break_match_hyps; try congruence.
-        repeat match goal with
-               | _ => progress cbn [orb]
-               | H : _ || _ = true |- _ =>
-                 apply orb_true_iff in H; destruct H
-               | H : _ = true |- _ => rewrite H
-               | _ => rewrite Bool.orb_true_r
-               | _ => reflexivity
-               end.
-        
-        
-        
-      cbn [valid_expr_bool cast_exempt negb andb] in *;
-      break_match_hyps;
-      cbn [valid_ident_bool valid_cast_exempt_bool
-                            valid_cast_bool
-                            translate_binop] in *;
-      repeat match goal with
-             | H : false = true |- _ => congruence
-             | H : true = false |- _ => congruence
-             | H : exists _, type.arrow _ _ = type.base _ |- _ =>
-               destruct H; congruence
-             | _ => progress subst
-             | H : _ && _ = true |- _ =>
-               apply andb_true_iff in H; destruct H
-             | H : _ && _ = false |- _ =>
-               apply andb_false_iff in H; destruct H
-             end.
-
-  Definition valid_ident_bool {t} (i : ident.ident t)
-    : type.for_each_lhs_of_arrow API.expr t -> (* argument expressions *)
-      bool :=
-    match i in ident.ident t0 return
-          type.for_each_lhs_of_arrow (@API.expr (fun _ => unit))
-                                     t0 -> bool with
-    | ident.fst _ _ => fun _ => true
-    | ident.snd _ _ => fun _ => true
-    | ident.Z_cast => fun _ => true
-    | ident.Z_cast2 => fun _ => true
-    | ident.List_nth_default base_Z =>
-      fun args =>
-        let '(d, (l, (i, _))) := args in
-        match i with
-        | expr.Ident _ (ident.Literal base.type.nat i) =>
-          true
-        | _ => false
-        end
-    | ident.Z_shiftr =>
-      fun args =>
-        let '(x, (n, _)) := args in
-        match n with
-        | expr.Ident _ (ident.Literal base.type.Z n) =>
-          is_bounded_by_bool n width_range
-        | _ => false
-        end
-    | ident.Z_truncating_shiftl =>
-      fun args =>
-        let '(s, (x, (n, _))) := args in
-        match s with
-        | expr.Ident _ (ident.Literal base.type.Z s) =>
-          match n with
-          | expr.Ident _ (ident.Literal base.type.Z n) =>
-            (Z.eqb s Semantics.width) && is_bounded_by_bool n width_range 
-          | _ => false
-          end
-        | _ => false
-        end
-    | ident.Z_mul_high =>
-      fun args =>
-        let '(s, (x, (y, _))) := args in
-        match s with
-        | expr.Ident _ (ident.Literal base.type.Z s) =>
-          Z.eqb s (2 ^ Semantics.width)
-        | _ => false
-        end
-    | i =>
-      fun _ =>
-        match translate_binop i with
-        | Some x => true
-        | None => false
-        end
-    end.
-
-  Definition valid_cast_exempt_bool {t}
-             (require_in_bounds : bool)
-             (e : @API.expr (fun _ => unit) t) : bool :=
-    match e with
-    | (expr.Ident type_Z (ident.Literal base.type.Z z)) =>
-      if require_in_bounds
-      then is_bounded_by_bool z max_range
-      else true 
-    | (expr.Ident type_nat (ident.Literal base.type.nat n)) =>
-      (* nats are only valid if not required to be in bounds
-         (in practice, this means only if they are an argument to
-         nth_default) *)
-      negb (require_in_bounds)
-    | expr.Var type_listZ x => true
-    | _ => false
-    end.
-
-  Definition valid_cast_bool
-             {t} (f : @API.expr (fun _ => unit) t) : bool :=
-    match f with
-    | expr.App
-        _ _ (expr.Ident _ ident.Z_cast)
-        (expr.Ident type_range (ident.Literal base.type.zrange r)) =>
-      range_good r
-    | expr.App
-        _ _ (expr.Ident _ ident.Z_cast2)
-        (expr.App
-           _ _
-           (expr.App
-              _ _ (expr.Ident _ (ident.pair _ _))
-              (expr.Ident type_range (ident.Literal base.type.zrange r1)))
-           (expr.Ident type_range (ident.Literal base.type.zrange r2))) =>
-      range_good r1 && range_good r2
-    | _ => false
-    end.
-
-  Fixpoint valid_expr_bool {t} (require_cast : bool)
-           (e : @API.expr (fun _ => unit) t) :
-    type.for_each_lhs_of_arrow API.expr t -> bool :=
-    if cast_exempt e
-    then fun _ => valid_cast_exempt_bool require_cast e
-    else if require_cast
-         then match e in expr.expr t0 return
-                    type.for_each_lhs_of_arrow _ t0 -> bool with
-              | expr.App (type.base _) _ f x =>
-                fun y =>
-                  if valid_cast_bool f
-                  then (valid_expr_bool false f (x, y))
-                         && (valid_expr_bool false x tt)
-                  else false
-              | _ => fun _ => false
-              end
-         else
-           match e in expr.expr t0 return
-                 type.for_each_lhs_of_arrow _ t0 -> bool with
-           | expr.App (type.base _) _ f x =>
-             fun y =>
-               let rc := require_cast_for_arg f in
-               (valid_expr_bool false f (x, y))
-                 && (valid_expr_bool rc x tt)
-           | expr.Ident _ i => valid_ident_bool i
-           | expr.Var type_Z x => fun _ => true
-           | expr.Var type_listZ x => fun _ => true
-           | _ => fun _ => false
-           end.
-
+                 | IH : forall binop_only shift_only _ _,
+                     if binop_only
+                     then False
+                     else if shift_only
+                          then False
+                          else _ |- _ =>
+                   specialize (IH false false); cbn in IH
+                 end.
+      { (* only_binop case *)
+        intros.
+        apply (valid_expr_binop_bool_impl1
+                 (t:=type_Z -> type_Z -> type_Z)); eauto. }
+      { (* only_shift case *)
+        intros.
+        apply (valid_expr_shift_bool_impl1
+                 (t:=type_Z -> type_Z -> type_Z)); eauto. }
+      { (* fully-applied binop case *)
+        intros.
+        apply (IHe1 true false); eauto. }
+      { (* fully-applied shift case *)
+        intros.
+        apply (IHe1 false true); eauto. }
+      { (* cast Z case *)
+        intros.
+        apply (valid_expr_App1_bool_impl1
+                 (t := type_Z -> type_Z)); eauto. }
+      { (* nth_default case *)
+        eauto using valid_expr_nth_default_bool_impl1. }
+      { (* fst/snd *)
+        intros.
+        apply (valid_expr_App1_bool_impl1
+                 (t := type_ZZ -> type_Z)); eauto. }
+      { (* cast ZZ *)
+        intros.
+        apply (valid_expr_App1_bool_impl1
+                 (t := type_ZZ -> type_ZZ)); eauto. } }
+    { break_match; try congruence. }
+  Qed.
 
   Lemma valid_expr_bool_impl1 {t} (e : API.expr t) :
     (exists b, t = type.base b) ->
-    forall rc args,
-      valid_expr_bool rc e args = true -> valid_expr rc e.
+    forall rc,
+      valid_expr_bool rc e = true -> valid_expr rc e.
   Proof.
-    induction e; intros;
-      cbn [valid_expr_bool cast_exempt negb andb] in *;
-      break_match_hyps;
-      cbn [valid_ident_bool valid_cast_exempt_bool
-                            valid_cast_bool
-                            translate_binop] in *;
-      repeat match goal with
-             | H : false = true |- _ => congruence
-             | H : true = false |- _ => congruence
-             | H : exists _, type.arrow _ _ = type.base _ |- _ =>
-               destruct H; congruence
-             | _ => progress subst
-             | H : _ && _ = true |- _ =>
-               apply andb_true_iff in H; destruct H
-             | H : _ && _ = false |- _ =>
-               apply andb_false_iff in H; destruct H
-             end.
-    { destruct rc;
-        constructor;
-        repeat match goal with
-               | H : is_bounded_by_bool _ _ = true |- _ =>
-                 rewrite H
-               | |- (_ || _)%bool = true => apply Bool.orb_true_iff
-               | _ => tauto
-               end. }
-    { destruct rc;
-        try constructor;
-        repeat match goal with
-               | H : false = true |- _ => congruence
-               | _ => progress cbn [negb] in *
-               | H : is_bounded_by_bool _ _ = true |- _ =>
-                 rewrite H
-               | |- (_ || _)%bool = true => apply Bool.orb_true_iff
-               | _ => tauto
-               end. }
-    { constructor. }
-    { break_match_hyps;
-        try constructor;
-        repeat match goal with
-               | H : false = true |- _ => congruence
-               end. }
-    2:{
-      
-
-
-      cbv [is_cast] in *.
-      break_match_hyps.
-      constructor. 
+    cbv [valid_expr_bool]; intros.
+    match goal with H : _ = true |- _ =>
+                    apply valid_expr_bool'_impl1 in H end.
+    eauto.
   Qed.
-
-  Lemma is_cast_literal_type {var t} (r : @API.expr var t) :
-
-    is_cast_literal r = true ->
-    t = type_range.
-  Proof.
-    cbv [is_cast_literal].
-    break_match; congruence.
-  Qed.
-
-  Lemma valid_cast_ident {var t} (r : @API.expr var t) :
-    is_cast_literal r = true ->
-    (match t as t0 return
-           expr.expr t0 -> Prop with
-     | type_range =>
-       fun r =>
-         r = expr.Ident (ident.Literal (t:=base.type.zrange) max_range)
-     | _ => fun _ => False
-     end) r.
-  Proof.
-    cbv [is_cast_literal].
-    break_match; try congruence.
-    destruct idc.
-
-  Lemma valid_cast_ident {t} (f : API.expr t) :
-    is_cast_ident f = true ->
-    (match t as t0 return
-           expr.expr t0 -> Prop with
-     | type.arrow s1 (type.arrow s2 d) =>
-       fun f =>
-         forall
-           (r : API.expr s1)
-           (x : API.expr s2)
-           (args : type.for_each_lhs_of_arrow API.expr d),
-           is_cast_literal r = true ->
-           valid_expr_bool false (expr.App f r) (x, args) = true ->
-           valid_expr true x ->
-           valid_expr true (expr.App (expr.App f r) x)
-     | _ => fun _ => False
-     end) f.
-  Proof.
-    cbv [is_cast_ident].
-    break_match; try congruence;
-      intros;
-      try match goal with
-          | H: @is_cast_literal _ _ type_range2 _ = true |- _ =>
-            apply is_cast_literal_type in H; congruence
-          end.
-    break_match_hyps; try congruence.
-    apply valid_cast_literal in H0
-    
-
-    2:{
-      intros.
-      apply valid_cast_literal in H0.
-      congruence.
-      exfalso.
-      clear H1.
-      remember type_ZZ.
-      cbv [is_cast_literal] in *.
-      break_match_hyps; try congruence.
-      destruct r; try congruence.
-      destruct idc; try congruence.
-      destruct t; try congruence.
-      { destruct idc0; try congruence.
-        destruct t0; try congruence.
-
-  Lemma valid_cast_impl1 {t} (f : API.expr t):
-    is_cast f = true ->
-    (match t as t0 return expr.expr t0 -> Prop with
-     | type.base _ => fun _ => False
-     | type.arrow s d =>
-       fun f =>
-         forall
-           (x : API.expr s)
-           (args : type.for_each_lhs_of_arrow API.expr d),
-           valid_expr_bool false f (x, args) = true ->
-           (* valid_expr_bool false x tt = true -> *)
-           valid_expr true (expr.App f x)
-     end) f.
-  Proof.
-    cbv [is_cast].
-    break_match; try congruence.
-    remember t.
-    repeat match goal with
-           | |- forall (_: match ?x with | _ => _ end = true), _ =>
-             destruct x; try congruence
-           | |- forall (_: (match ?x with | _ => _ end) _ = true), _ =>
-             destruct x; try congruence
-           | |- forall (_: (match ?x with | _ => _ end) _ _ = true), _ =>
-             destruct x; try congruence
-           end.
-    { break_match.
-      Set Printing Implicit.
-      cbv [is_cast_ident].
-      destruct f1.
-    destruct f; try congruence.
-    destruct s; try congruence.
-    destruct t; try congruence.
-    { destruct t; try congruence. 
-    destruct f1.
-  Lemma is_cast_ident_base
-             {var s d} (e : @API.expr var (s -> d)) :
-    (exists b, d = type.base b) ->
-    is_cast_ident e = false.
-  Proof.
-    cbv [is_cast_ident].
-    destruct e; try reflexivity.
-    destruct idc; try reflexivity.
-    break_match; try congruence. 
-    destruct e; cbn.
-    
-
-
-
-  Definition valid_cast_postcondition {t}
-    : API.expr t -> Prop :=
-    match t as t0 return expr.expr t0 -> Prop with
-     | type.base _ => fun _ => False
-     | type.arrow s d =>
-       fun f =>
-         forall
-           (x : API.expr s)
-           (args : type.for_each_lhs_of_arrow API.expr d),
-           valid_expr_bool false f (x, args) = true ->
-           (* valid_expr_bool false x tt = true -> *)
-           valid_expr true (expr.App f x)
-     end. 
-
-  Lemma valid_cast_apprange {t1 t2}
-        (f : API.expr t1)
-        (r : API.expr t2) :
-    match f with
-    | expr.Ident _ ident.Z_cast =>
-      match r with
-      | expr.Ident _ (ident.Literal base.type.zrange r) =>
-        range_good r
-      | _ => false
-      end
-    | _ => false
-    end = true ->
-    (match t1 as t3 return
-           expr.expr t3 -> expr.expr t2 -> Prop with
-     | type.arrow type_range d =>
-       fun f =>
-         match t2 as t4 return expr.expr t4 -> Prop with
-         | type_range =>
-           fun r =>
-             valid_cast_postcondition (expr.App f r)
-         | _ => fun _ => False
-         end
-     | _ => fun _ _ => False
-     end) f r.
-  Proof.
-    destruct f; try congruence.
-    destruct idc; try congruence.
-    destruct r; try congruence.
-    destruct idc; try congruence.
-    destruct t; try congruence.
-    cbn [valid_cast_postcondition]; intros.
-    cbn [valid_expr_bool cast_exempt require_cast_for_arg] in *.
-    rewrite Bool.andb_false_r in *. congruence.
-  Qed.
-
-  (*
-  Lemma valid_cast2_apppair {t1 t2}
-        (f : API.expr t1)
-        (r : API.expr t2) :
-    match f with
-    | expr.App
-        _ _ (expr.Ident type_range2 (ident.pair _ _))
-        (expr.Ident _ (ident.Literal base.type.zrange r1)))
-        (expr.Ident _ (ident.Literal base.type.zrange r2)) =>
-      range_good r1 && range_good r2
-    | _ => false
-    end
-    | _ => false
-    end = true ->
-    (match t1 as t3 return
-           expr.expr t3 -> expr.expr t2 -> Prop with
-     | type.arrow type_range2 d =>
-       fun f =>
-         match t2 as t4 return expr.expr t4 -> Prop with
-         | type_range2 =>
-           fun r =>
-             valid_cast_postcondition (expr.App f r)
-         | _ => fun _ => False
-         end
-     | _ => fun _ _ => False
-     end) f r.
-  Proof.
-*)
-
-  Lemma of_apprange {var d}
-        (P : forall d,
-            API.expr (var:=var) (type_range -> d) ->
-            API.expr (var:=var) type_range -> Prop)
-        (f : API.expr (type_range -> d))
-        (x : API.expr type_range):
-    (forall t1 t2
-            (f' : API.expr t1)
-            (x' : API.expr t2),
-        (match t1 as t3
-               return expr.expr t3 ->
-                      expr.expr t2 -> Prop with
-         | type.arrow type_range d0 =>
-           fun f'' : API.expr (type_range -> d0) =>
-             match t2 as t4
-                   return expr.expr t4 -> Prop with
-             | type_range =>
-               fun x'' => P d0 f'' x''
-             | _ => fun _ => False
-             end
-         | _ => fun _ _ => False
-         end) f' x') ->
-    P _ f x.
-  Proof.
-    let H := fresh in
-    intro H; specialize (H _ _ f x).
-    assumption.
-  Qed.
-
-  (*
-    match f with
-    | Ident (s -> d) _ => 
-      match x with
-      | _ =>
-      end
-    end = true ->
-    P (f @ x)
-    
-
-
-    match f with
-    | Ident (s -> d) _ => 
-      match x with
-      | _ =>
-      end
-    end = true ->
-    P e
-
-  *)
-  Lemma of_apprange' {var d}
-        (pre : forall t2 t1, (* important to take t2 first *)
-            API.expr (var:=var) t1 ->
-            API.expr (var:=var) t2 -> bool)
-        (P : forall t,
-            API.expr (var:=var) t -> Prop)
-        (f : API.expr (type_range -> d))
-        (x : API.expr type_range):
-    (forall t1 t2 f' x',
-        pre t2 t1 f' x' = true ->
-        (match t1 as t3 return
-               expr.expr t3 -> expr.expr t2 -> Prop with
-         | type.arrow type_range d =>
-           fun f'' =>
-             match t2 as t4 return expr.expr t4 -> Prop with
-             | type_range =>
-               fun x'' =>
-                 P _ (expr.App f'' x'')
-             | _ => fun _ => False
-             end
-         | _ => fun _ _ => False
-         end) f' x') ->
-    (pre _ _ f x = true) ->
-    P d (expr.App f x).
-  Proof.
-    let H := fresh in
-    intro H; specialize (H _ _ f x).
-    assumption.
-  Qed.
-  Lemma of_apprange2 {var d}
-        (pre : forall t2 t1, (* important to take t2 first *)
-            API.expr (var:=var) t1 ->
-            API.expr (var:=var) t2 -> bool)
-        (P : forall t,
-            API.expr (var:=var) t -> Prop)
-        (f : API.expr (type_range2 -> d))
-        (x : API.expr type_range2):
-    (forall t1 t2 f' x',
-        pre t2 t1 f' x' = true ->
-        (match t1 as t3 return
-               expr.expr t3 -> expr.expr t2 -> Prop with
-         | type.arrow type_range2 d =>
-           fun f'' =>
-             match t2 as t4 return expr.expr t4 -> Prop with
-             | type_range2 =>
-               fun x'' =>
-                 P _ (expr.App f'' x'')
-             | _ => fun _ => False
-             end
-         | _ => fun _ _ => False
-         end) f' x') ->
-    (pre _ _ f x = true) ->
-    P d (expr.App f x).
-  Proof.
-    let H := fresh in
-    intro H; specialize (H _ _ f x).
-    assumption.
-  Qed.
-  
-  (*
-  Lemma valid_cast2_apprange {t1 t2}
-        (f : API.expr t1)
-        (r : API.expr t2) :
-    match f with
-    | expr.Ident _ ident.Z_cast2 =>
-      match r with
-      | expr.App
-          _ _ (expr.App
-                 _ _ (expr.Ident type_range2 (ident.pair _ _))
-                 (expr.Ident _ (ident.Literal base.type.zrange r1)))
-          (expr.Ident _ (ident.Literal base.type.zrange r2)) =>
-        range_good r1 && range_good r2
-      | _ => false
-      end
-    | _ => false
-    end = true ->
-    (match t1 as t3 return
-           expr.expr t3 -> expr.expr t2 -> Prop with
-     | type.arrow type_range2 d =>
-       fun f =>
-         match t2 as t4 return expr.expr t4 -> Prop with
-         | type_range2 =>
-           fun r =>
-             valid_cast_postcondition (expr.App f r)
-         | _ => fun _ => False
-         end
-     | _ => fun _ _ => False
-     end) f r.
-  Proof.
-    repeat match goal with
-           | |- forall (_: match ?x with | _ => _ end = true), _ =>
-             destruct x; try congruence
-           | |- forall (_: (match ?x with | _ => _ end) _ = true), _ =>
-             destruct x; try congruence
-           | |- forall (_: (match ?x with | _ => _ end) _ _ = true), _ =>
-             destruct x; try congruence
-           end.
-    eapply of_apprange.
-    destruct r1.
-    destruct f; try congruence.
-    destruct idc; try congruence.
-    destruct r; try congruence.
-    destruct idc; try congruence.
-    destruct t; try congruence.
-    cbn [valid_cast_postcondition]; intros.
-    cbn [valid_expr_bool cast_exempt require_cast_for_arg] in *.
-    rewrite Bool.andb_false_r in *. congruence.
-  Qed.
-*)
-
-  Lemma valid_cast_impl1 {t}
-        (f : API.expr t) :
-    is_cast f = true ->
-    valid_cast_postcondition f.
-  Proof.
-    cbv [is_cast].
-    repeat match goal with
-           | |- forall (_: match ?x with | _ => _ end = true), _ =>
-             destruct x; try congruence
-           | |- forall (_: (match ?x with | _ => _ end) _ = true), _ =>
-             destruct x; try congruence
-           | |- forall (_: (match ?x with | _ => _ end) _ _ = true), _ =>
-             destruct x; try congruence
-           end.
-    { match goal with
-      | e1 : API.expr (type.arrow ?s ?d), e2 : API.expr ?t2
-        |- ?pre = true -> ?Q =>
-        let pre :=
-            lazymatch (eval pattern e2 in pre) with ?f _ => f end in
-        let pre :=
-            lazymatch (eval pattern e1 in pre) with ?f _ => f end in
-        let pre :=
-            lazymatch (eval pattern (type.arrow s d) in pre) with ?f _ => f end in
-        let pre :=
-            lazymatch (eval pattern t2 in pre) with ?f _ => f end in
-        change (pre _ _ e1 e2 = true -> Q);
-          intro;
-          apply (of_apprange' pre); [ | assumption ]
-      end.
-      clear. intros *.
-      repeat match goal with
-             | |- forall (_: match ?x with | _ => _ end = true), _ =>
-               destruct x; try congruence
-             | |- forall (_: (match ?x with | _ => _ end) _ = true), _ =>
-               destruct x; try congruence
-             | |- forall (_: (match ?x with | _ => _ end) _ _ = true), _ =>
-               destruct x; try congruence
-             end.
-      cbn [valid_cast_postcondition]; intros.
-      cbn [valid_expr_bool cast_exempt require_cast_for_arg
-                           valid_ident_bool andb] in *.
-      congruence. }
-    { match goal with
-      | e1 : API.expr (type.arrow ?s ?d), e2 : API.expr ?t2
-        |- ?pre = true -> ?Q =>
-        let pre :=
-            lazymatch (eval pattern e2 in pre) with ?f _ => f end in
-        let pre :=
-            lazymatch (eval pattern e1 in pre) with ?f _ => f end in
-        let pre :=
-            lazymatch (eval pattern (type.arrow s d) in pre) with ?f _ => f end in
-        remember pre end.
-
-      match type of Heqb with _ =
-                              (fun t e (e0 : API.expr type_range2) =>
-                                 ?f) =>
-                              let pre :=
-                                  constr:(fun t t' e (e0 : API.expr t') =>
-                                     f) in
-                              idtac pre
-      end.
-      
-                              idtac f end.
-                              let f := lazymatch (eval pattern type_range2 in x) with ?f _ => f end in idtac f end.
-          idtac t2 pre end.
-        let pre :=
-            lazymatch (eval pattern t2 in pre) with ?f _ => f end in
-          idtac pre end.
-        change (pre _ _ e1 e2 = true -> Q);
-          intro;
-          apply (of_apprange' pre); [ | assumption ]
-      end.
-      clear. intros *.
-      repeat match goal with
-             | |- forall (_: match ?x with | _ => _ end = true), _ =>
-               destruct x; try congruence
-             | |- forall (_: (match ?x with | _ => _ end) _ = true), _ =>
-               destruct x; try congruence
-             | |- forall (_: (match ?x with | _ => _ end) _ _ = true), _ =>
-               destruct x; try congruence
-             end.
-      cbn [valid_cast_postcondition]; intros.
-      cbn [valid_expr_bool cast_exempt require_cast_for_arg
-                           valid_ident_bool andb] in *.
-      congruence. }
-        
-        intros. subst b.
-      pose proof (fun d => @of_apprange' _ d b) as HAPP.
-      intro H.
-      apply HAPP.
-      apply HAPP in H.
-      apply (of_apprange' b).
-      apply H.
-      match goal with
-      | |- ?P -> ?Q =>
-        let pre :=
-            lazymatch (eval pattern f1 in P) with ?f _ => f end in
-        let pre :=
-            lazymatch (eval pattern (type.arrow type_range (type.arrow type_Z type_Z)) in pre) with ?f _ => f end in
-        idtac pre
-      end.
-      
-    (pre _ _ f x = true) ->
-    P d (expr.App f x).
-      eapply of_apprange'; eauto; intros.
-      break_match.
-    { let H := fresh in
-      intro H; apply valid_cast_apprange in H.
-      assumption. }
-    { 
-    destruct f; try congruence.
-    destruct s; try congruence.
-    destruct t; try congruence.
-    { destruct t; try congruence.
-      destruct d; try congruence.
-      destruct d1; try congruence.
-      destruct t; try congruence.
-      destruct t; try congruence.
-      destruct d2; try congruence.
-      destruct t; try congruence.
-      destruct t; try congruence.
-      intros.
-      apply valid_cast_apprange in H.
-      apply H. }
-    { destruct t1; try congruence.
-      destruct t; try congruence.
-      destruct d; try congruence.
-      destruct d1; try congruence.
-      destruct t; try congruence.
-      destruct t; try congruence.
-      destruct d2; try congruence.
-      destruct t; try congruence.
-      destruct t; try congruence.
-      intros.
-      apply valid_cast_apprange in H.
-      apply H. }
-
+End Expr.
